src/BuiltinSem.v
@@ -1,0 +1,74 @@
+Require Import List.
+Require Import String.
+
+Require Import Coqlib.
+
+Require Import AST.
+Require Import Builtins.
+Require Import Values.
+Require Import Integers.
+
+Open Scope string.
+
+Fixpoint make_arg_list (n : nat) : list Expr :=
+  match n with
+  | O => nil
+  | S n' => (EVar (Z.of_nat n, "")) :: make_arg_list n'
+  end.
+
+Fixpoint iter {A : Type} (n : nat) (f : nat -> A -> A) (b : A) : A :=
+  match n with
+  | O => b
+  | S n' => f n (iter n' f b)
+  end.
+
+Definition mb (num_type_args : nat) (num_args : nat) (b : builtin) : Expr :=
+  let l := make_arg_list (num_args + num_type_args) in 
+  let raw_e := iter num_args (fun n => fun x => EAbs (Z.of_nat n, "") x) (EBuiltin b l) in
+  let t_e := iter num_type_args (fun n => fun x => ETAbs ((Z.of_nat (n + num_args )), "") x) raw_e in
+  t_e.
+
+
+(* table of builtins, along with their type and val level arity *)
+Definition table : list (string * Expr) :=
+  ("demote", mb 2 0 Demote) ::
+  ("+", mb 1 2 Plus) ::
+  ("-", mb 1 2 Minus) ::
+  ("negate", mb 1 1 Neg) ::
+  ("==", mb 1 2 Eq) ::
+  nil.
+
+(* Here we have the semantics of all builtins *)
+Inductive eval_builtin : builtin -> list val -> val -> Prop :=
+| eval_plus :
+    forall {w : nat} {nz : w <> O} (b1 b2 b3 : BitV w) t,
+      b3 = @add w nz b1 b2 ->
+      eval_builtin Plus (t :: (bits b1) :: (bits b2) :: nil) (bits b3)
+| eval_eq :
+    forall {w : nat} (b1 b2 : BitV w) (b : bool) t,
+      b = @eq w b1 b2 ->
+      eval_builtin Eq (t :: (bits b1) :: (bits b2) :: nil) (bit b)
+| eval_neg :
+    forall {w : nat} {nz : w <> O} (b1 b2 : BitV w) t,
+      b2 = @neg w nz b1 ->
+      eval_builtin Neg (t :: (bits b1) :: nil) (bits b2)
+| eval_demote :
+    forall {ws : nat} {nz : ws <> O} (w n : Z) (b : BitV ws),
+      ws = Z.to_nat w ->
+      b = @repr ws nz n ->
+      eval_builtin Demote ((typ (TCon (TC (TCNum n)) nil)) :: (typ (TCon (TC (TCNum w)) nil)) :: nil) (bits b)
+.
+
+Fixpoint lookup {A : Type} (s : string) (t : list (string * A)) : option A :=
+  match t with
+  | nil => None
+  | (n,a) :: r => if string_dec n s then Some a else lookup s r
+  end.
+
+Definition find_builtin (s : string) : option Expr :=
+  lookup s table.
+
+Definition lookup_prim (id : ident) : option Expr :=
+  let (_,n) := id in
+  find_builtin n.
+              
