src/Values.v
@@ -1,0 +1,15 @@
+Require Import AST.
+Require Import String.
+
+Inductive val :=
+| bit (b : bool) (* Can we ever get this now? *)
+| bits {n} (b : BitV n) (* bitvector *)
+| close (id : ident) (e : Expr) (E : ident -> option val)  (* closure *)
+| tuple (l : list val) (* heterogeneous tuples *)
+| rec (l : list (string * val))
+| vcons (v : val) (e : Expr) (E : ident -> option val) (* lazy list: first val computed, rest is thunked *)
+| vnil (* empty list *)
+| vcomp (e : Expr) (E : ident -> option val) (l : list (list Match)) (* lazy list comprehension *)
+| typ (t : Typ) (* type value, used to fill in type variables *)
+| tclose (id : ident) (e : Expr) (E : ident -> option val) (* type closure *)
+.
